src/Pyrosome/Tools/EGraph/Test.v
@@ -1,0 +1,158 @@
+(* Some basic tests of the egraph machinery *)
+Require Import Lists.List Strings.String.
+Import ListNotations.
+Open Scope list.
+
+
+From coqutil Require Import Map.Interface.
+
+From Utils Require Import Utils UnionFind Monad ExtraMaps.
+From Utils.EGraph Require Import Defs Semantics QueryOpt.
+Import Monad.StateMonad.
+From Pyrosome.Theory Require Import Core.
+Import Core.Notations.
+From Pyrosome.Tools.EGraph Require Import Defs.
+Import StringInstantiation.
+
+Notation log_rule := (log_rule string string).
+
+(* TODO: make this available in other places than the tests *)
+Declare Custom Entry logrule.
+Declare Custom Entry atom.
+Declare Custom Entry unification.
+Declare Scope log_scope.
+Bind Scope log_scope with log_rule.
+Delimit Scope log_scope with log.
+
+(*TODO: move to defining file*)
+Arguments Build_log_rule {idx symbol}%type_scope
+  (query_vars query_clauses write_clauses write_unifications)%list_scope.
+
+Notation "!! x" := x (at level 60, x custom logrule) : log_scope.
+
+(*TODO: compute query vars for convenience*)
+Notation "wc , .. , wc' | wu , .. , wu' :- qc , .. , qc' [ var .. var' ]" :=
+  (Build_log_rule
+     (cons var' .. (cons var nil) ..)
+     (cons qc' .. (cons qc nil) ..)
+     (cons wc' .. (cons wc nil) ..)
+     (cons wu' .. (cons wu nil) ..))
+    (in custom logrule at level 60,
+        wc custom atom at level 50,
+        wu custom unification at level 50,
+        qc custom atom at level 50,
+        var constr at level 0).
+
+Notation "wc , .. , wc' :- qc , .. , qc' [ var .. var' ]" :=
+  (Build_log_rule
+     (cons var' .. (cons var nil) ..)
+     (cons qc' .. (cons qc nil) ..)
+     (cons wc' .. (cons wc nil) ..)
+     [])
+    (in custom logrule at level 60,
+        wc custom atom at level 50,
+        qc custom atom at level 50,
+        var constr at level 0).
+
+Notation "wc , .. , wc' | wu , .. , wu' :- [ var .. var' ]" :=
+  (Build_log_rule
+     (cons var' .. (cons var nil) ..)
+     nil
+     (cons wc' .. (cons wc nil) ..)
+     (cons wu' .. (cons wu nil) ..))
+    (in custom logrule at level 60,
+        wc custom atom at level 50,
+        wu custom unification at level 50,
+        var constr at level 0).
+
+Notation "wc , .. , wc' :- [ var .. var' ]" :=
+  (Build_log_rule
+     (cons var' .. (cons var nil) ..)
+     nil
+     (cons wc' .. (cons wc nil) ..)
+     [])
+    (in custom logrule at level 60,
+        wc custom atom at level 50,
+        var constr at level 0).
+
+
+(*TODO: compute query vars for convenience*)
+Notation "wc , .. , wc' | wu , .. , wu' :- qc , .. , qc'" :=
+  (Build_log_rule
+     nil
+     (cons qc' .. (cons qc nil) ..)
+     (cons wc' .. (cons wc nil) ..)
+     (cons wu' .. (cons wu nil) ..))
+    (in custom logrule at level 60,
+        wc custom atom at level 50,
+        wu custom unification at level 50,
+        qc custom atom at level 50).
+
+Notation "wc , .. , wc' :- qc , .. , qc'" :=
+  (Build_log_rule
+     nil
+     (cons qc' .. (cons qc nil) ..)
+     (cons wc' .. (cons wc nil) ..)
+     [])
+    (in custom logrule at level 60,
+        wc custom atom at level 50,
+        qc custom atom at level 50).
+
+Notation "wc , .. , wc' | wu , .. , wu' :-" :=
+  (Build_log_rule
+     nil
+     nil
+     (cons wc' .. (cons wc nil) ..)
+     (cons wu' .. (cons wu nil) ..))
+    (in custom logrule at level 60,
+        wc custom atom at level 50,
+        wu custom unification at level 50).
+
+Notation "wc , .. , wc' :-" :=
+  (Build_log_rule
+     nil
+     nil
+     (cons wc' .. (cons wc nil) ..)
+     [])
+    (in custom logrule at level 60,
+        wc custom atom at level 50).
+
+Notation "f a .. a' -> r" :=
+  (Build_atom f (cons a' .. (cons a nil) ..) r)
+    (in custom atom at level 50,
+        f constr at level 0,
+        a constr at level 0,
+        r constr at level 0).
+
+Notation "f -> r" :=
+  (Build_atom f nil r)
+    (in custom atom at level 50,
+        f constr at level 0,
+        r constr at level 0).
+
+Notation "a = b" :=
+  (a,b)
+    (in custom unification at level 50, a constr at level 0,
+    b constr at level 0).
+           
+Definition example1 : list log_rule :=
+  [!! "dog" -> "d" :-;
+   !! "cat" -> "c" :-;
+   !! "canine" "x" -> "t" :- "dog" -> "x" [ "x" ];
+   !! "animal" "x" -> "t" :- "dog" -> "x" [ "x" ];
+   !! "animal" "x" -> "t" :- "cat" -> "x" [ "x" ]
+  ]%log.
+
+
+Definition ex1_set :=
+  Eval vm_compute in
+    QueryOpt.build_rule_set _ _ string_succ "v0" _ string_trie_map
+      _ string_trie_map example1.
+
+Definition ex1_graph :=
+  Eval vm_compute in
+    (saturate_until string_succ "v0"
+       (@PositiveInstantiation.pt_spaced_intersect) ex1_set (Mret false) 10
+       (empty_egraph default)).
+
+(*TODO: test queries*)
